statics.v
@@ -1,20 +1,19 @@
 Require Import syntax.
 Require Import substitution.
 From stdpp Require Import gmap.
-From stdpp Require Import set.
 
-Definition set_add {T} (s : set T) (t : T) := set_union s (set_singleton t).
+(* pg. 140-141 *)
 
-Inductive WellTTyped : set type -> type -> Prop :=
-  | TypT th t : WellTTyped (set_add th (Typ t)) (Typ t)
+Inductive WellTTyped : gset type -> type -> Prop :=
+  | TypT th t : WellTTyped (th ∪ {[Typ t]}) (Typ t)
   | ArrT th tau1 tau2 : WellTTyped th tau1 -> WellTTyped th tau2 -> WellTTyped th (Arr tau1 tau2)
-  | AllT th t tau : WellTTyped (set_add th (Typ t)) tau -> WellTTyped th (All t tau)
+  | AllT th t tau : WellTTyped (th ∪ {[Typ t]}) tau -> WellTTyped th (All t tau)
   .
 
-Inductive WellTyped : set type -> gmap var type -> expr -> type -> Prop :=
+Inductive WellTyped : gset type -> gmap var type -> expr -> type -> Prop :=
   | VarT th g x tau : WellTyped th (<[x:=tau]>g) (Var x) tau 
   | LamT th c e x tau tau' : WellTyped th (<[x:=tau]>c) e tau' -> WellTyped th c (Lam x tau e) (Arr tau tau')
   | AppT th c e1 e2 t t2 : WellTyped th c e1 (Arr t2 t) -> WellTyped th c e2 t2 -> WellTyped th c (App e1 e2) t
-  | Lam2T g th e t tau : WellTyped (set_add th (Typ t)) g e tau -> WellTyped th g (Lam2 t e) (All t tau)
+  | Lam2T g th e t tau : WellTyped (th ∪ {[Typ t]}) g e tau -> WellTyped th g (Lam2 t e) (All t tau)
   | App2T th g e t tau tau' : WellTyped th g e (All t tau') -> WellTTyped th tau -> WellTyped th g (App2 e tau) (subst_t_t tau' tau t)
   .
