substitution.v
@@ -1,51 +1,53 @@
 Require Import syntax.
 From stdpp Require Import gmap.
-From stdpp Require Import set.
-
-
-Global Instance set_elem_dec {T} (x:T) (xs:set T) : Decision (set_elem_of x xs).
-Proof. Admitted.
 
 Global Instance type_dec : EqDecision type.
 Proof. solve_decision. Qed.
 
-(* Expression substitution *)
-Fixpoint FVE e := 
+Fixpoint FVE e : gset var := 
   match e with
-  | Var x => set_singleton x 
-  | Lam x t e => set_difference (FVE e) (set_singleton (x))
-  | App e1 e2 => set_union (FVE e1) (FVE e2)
+  | Var x => {[x]} 
+  | Lam x t e => FVE e ∖ {[x]}
+  | App e1 e2 => FVE e1 ∪ FVE e2
   | Lam2 t e => FVE e
   | App2 e t => FVE e
   end.
 
-Fixpoint BVE e :=
+Fixpoint BVE e : gset var :=
  match e with
-  | Var x => set_empty
-  | Lam x t e => set_union (BVE e) (set_singleton (x))
-  | App e1 e2 => set_union (BVE e1) (BVE e2)
+  | Var x => ∅
+  | Lam x t e => BVE e ∪ {[x]}
+  | App e1 e2 => BVE e1 ∪ BVE e2
   | Lam2 t e => BVE e
   | App2 e t => BVE e
   end.
 
-Fixpoint subst_e_e e' e x :=
+Fixpoint subst_e_e e' e x : expr :=
   match e' with
   | Var x' => if decide (x' = x) then e else Var x' 
-  | Lam y tau e'' => if decide (y <> x /\ (not (set_elem_of y (FVE e)))) then Lam y tau (subst_e_e e'' e x) else Lam y tau e''
+  | Lam y tau e'' => if decide (y <> x /\ (y ∉ FVE e)) then Lam y tau (subst_e_e e'' e x) else Lam y tau e''
   | App e1 e2 => App (subst_e_e e1 e x) (subst_e_e e2 e x)
   | Lam2 t e'' => Lam2 t (subst_e_e e'' e x)
   | App2 e'' tau => App2 (subst_e_e e'' e x) tau
   end.
 
-Lemma none_subst_e e' e x : not (set_elem_of x (FVE e')) -> subst_e_e e' e x = e'.
+Lemma difference_nin (x y : var) (s : gset var) : x ∈ s -> y ≠ x -> x ∈ s ∖ {[y]}.
+Proof.
+  intros.
+  apply elem_of_difference. split.
+  - apply H.
+  - unfold not. intros. apply H0. apply elem_of_singleton in H1. rewrite H1. reflexivity.
+Qed.
+
+Lemma none_subst_e e' e x : x ∉ FVE e' -> subst_e_e e' e x = e'.
 Proof.
   intros HIn. 
   induction e'. 
   - simpl. destruct (decide (x0 = x)).
-    + unfold not in HIn. assert (False). { apply HIn. subst. simpl. done. } contradiction.
+    + unfold not in HIn. assert (False). { apply HIn. subst. simpl. apply elem_of_singleton. reflexivity. } contradiction.
     + reflexivity. 
-  - simpl. destruct (decide (x0 ≠ x ∧ (not (set_elem_of x0 (FVE e))))).
-    + destruct a. rewrite IHe'. reflexivity. unfold not in *. intros. apply HIn. done.
+  - simpl. destruct (decide (x0 ≠ x ∧ (x0 ∉ (FVE e)))).
+    + destruct a. rewrite IHe'. reflexivity. unfold not in *. intros. apply HIn. simpl. apply difference_nin. apply H1. unfold not. apply H.
     + reflexivity. 
   - simpl. rewrite IHe'1. rewrite IHe'2. reflexivity.
     + unfold not in *. intros. apply HIn. simpl. apply elem_of_union. right. apply H.
@@ -55,60 +57,59 @@ Proof.
 Qed.
 
 (* Type Substitution *)
-Fixpoint FVT t :=
+Fixpoint FVT t : gset var :=
   match t with
-  | Typ t => set_singleton t
-  | Arr tau1 tau2 => set_union (FVT tau1) (FVT tau2)
-  | All t tau => set_difference (FVT tau) (set_singleton t)
+  | Typ t => {[t]}
+  | Arr tau1 tau2 => FVT tau1 ∪ FVT tau2
+  | All t tau => FVT tau ∖  {[t]}
   end. 
 
-Fixpoint BVT t :=
+Fixpoint BVT t : gset var :=
   match t with
-  | Typ t => set_empty
-  | Arr tau1 tau2 => set_union (BVT tau1) (BVT tau2)
-  | All t tau => set_union (BVT tau) (set_singleton t)
+  | Typ t => ∅
+  | Arr tau1 tau2 => BVT tau1 ∪ BVT tau2
+  | All t tau => BVT tau ∪ {[t]}
   end.
 
-
-Fixpoint subst_t_t (tau':type) (tau:type) t :=
+Fixpoint subst_t_t (tau':type) (tau:type) t : type :=
   match tau' with
   | Typ t' => if decide (t = t') then tau else tau'
   | Arr tau1 tau2 => Arr (subst_t_t tau1 tau t) (subst_t_t tau2 tau t)
-  | All t' tau'' => if decide (t <> t' /\ (not (set_elem_of t' (FVT tau)))) then All t' (subst_t_t tau'' tau t) else All t' tau''
+  | All t' tau'' => if decide (t <> t' /\ t' ∉ FVT tau) then All t' (subst_t_t tau'' tau t) else All t' tau''
   end.
 
-Lemma none_subst_t tau' tau t : not (set_elem_of t (FVT tau')) -> subst_t_t tau' tau t = tau'.
+Lemma none_subst_t tau' tau t : t ∉ FVT tau' -> subst_t_t tau' tau t = tau'.
 Proof.
   intros HIn. 
   induction tau'.
   - simpl. destruct (decide (t = t0)).
-    + subst. unfold not in HIn. assert (False). { apply HIn. done. } contradiction.
+    + subst. unfold not in HIn. assert (False). { apply HIn. simpl. apply elem_of_singleton. reflexivity. } contradiction.
     + reflexivity.
   - simpl. rewrite IHtau'1. rewrite IHtau'2. reflexivity.
     + unfold not in *. intros. apply HIn. simpl. apply elem_of_union. right. apply H.
     + unfold not in *. intros. apply HIn. simpl. apply elem_of_union. left. apply H.
-  - simpl. destruct (decide (t ≠ t0 ∧ ¬ set_elem_of t0 (FVT tau))).
-    + destruct a. rewrite IHtau'. reflexivity. unfold not in *. intros. apply HIn. simpl. apply elem_of_difference. split. apply H1. unfold not. intros. apply H. inversion H2. reflexivity.
+  - simpl. destruct (decide (t ≠ t0 ∧ t0 ∉ FVT tau)).
+    + destruct a. rewrite IHtau'. reflexivity. unfold not in *. intros. apply HIn. simpl. apply elem_of_difference. split. apply H1. unfold not. intros. apply H. apply elem_of_singleton in H2. rewrite H2. reflexivity.
     + reflexivity.
 Qed.
 
 (* Type/Expressions *)
-Fixpoint FVET e : set var := 
+Fixpoint FVET e : gset var := 
   match e with
-  | Var x => set_empty
-  | Lam x tau e => set_union (FVET e) (FVT tau) 
-  | App e1 e2 => set_union (FVET e1) (FVET e2)
-  | Lam2 t e => set_difference (FVET e) (set_singleton t)
-  | App2 e tau => set_union (FVET e) (FVT tau) 
+  | Var x => ∅
+  | Lam x tau e => FVET e ∪ FVT tau 
+  | App e1 e2 => FVET e1 ∪ FVET e2
+  | Lam2 t e => FVET e ∖ {[t]}
+  | App2 e tau => FVET e ∪ FVT tau 
   end.
 
-Fixpoint BVET e : set var :=
+Fixpoint BVET e : gset var :=
  match e with
-  | Var x => set_empty
-  | Lam x tau e => set_union (BVET e) (BVT tau)
-  | App e1 e2 => set_union (BVET e1) (BVET e2)
-  | Lam2 t e => set_union (set_singleton t) (BVE e)
-  | App2 e tau => set_union (BVE e) (BVT tau)
+  | Var x => ∅
+  | Lam x tau e => BVET e ∪ BVT tau
+  | App e1 e2 => BVET e1 ∪ BVET e2
+  | Lam2 t e => {[t]} ∪ BVE e
+  | App2 e tau => BVE e ∪ BVT tau
   end.
 
 Fixpoint subst_e_t e' (tau:type) (t:var) :=
@@ -116,11 +117,11 @@ Fixpoint subst_e_t e' (tau:type) (t:var) :=
   | Var x => Var x
   | Lam x tau' e => Lam x (subst_t_t tau' tau t) (subst_e_t e tau t)
   | App e1 e2 => App (subst_e_t e1 tau t) (subst_e_t e2 tau t) 
-  | Lam2 t' e => if decide (t <> t' /\ (not (set_elem_of t' (FVET e)))) then Lam2 t' (subst_e_t e tau t) else Lam2 t' e
+  | Lam2 t' e => if decide (t <> t' /\ t' ∉ FVET e) then Lam2 t' (subst_e_t e tau t) else Lam2 t' e
   | App2 e tau' => App2 (subst_e_t e tau t) (subst_t_t tau' tau t)
   end.
 
-Lemma none_subst_et e tau t : not (set_elem_of t (FVET e)) -> subst_e_t e tau t = e.
+Lemma none_subst_et e tau t : t ∉ FVET e -> subst_e_t e tau t = e.
 Proof.
   intros HIn. 
   induction e.
@@ -131,8 +132,8 @@ Proof.
   - simpl. rewrite IHe1. rewrite IHe2. reflexivity.
     unfold not in *. intros. apply HIn. simpl. apply elem_of_union. right. apply H.
     unfold not in *. intros. apply HIn. simpl. apply elem_of_union. left. apply H.
-  - simpl. destruct (decide (t ≠ t0 ∧ ¬ set_elem_of t0 (FVET e))).
-    + rewrite IHe. reflexivity. destruct a. simpl in HIn. unfold not in *. intros. apply HIn. simpl. apply elem_of_difference. split. apply H1. unfold not. intros. apply H. inversion H2. reflexivity.
+  - simpl. destruct (decide (t ≠ t0 ∧ t0 ∉ FVET e)).
+    + rewrite IHe. reflexivity. destruct a. simpl in HIn. unfold not in *. intros. apply HIn. simpl. apply elem_of_difference. split. apply H1. unfold not. intros. apply H. apply elem_of_singleton in H2. rewrite H2. reflexivity.
     + reflexivity.
   - simpl. rewrite IHe. rewrite none_subst_t. reflexivity. 
     unfold not in *. intros. apply HIn. simpl. apply elem_of_union. right. apply H.
