syntax.v
@@ -1,9 +1,10 @@
 From stdpp Require Import gmap.
-From stdpp Require Import set.
 
-Definition var := nat.
+Definition var := positive.
 Global Instance var_dec : EqDecision var.
 Proof. solve_decision. Qed.
+
+(* Pg. 140 *)
 
 Inductive type :=
   | Typ (t : var)
@@ -18,3 +19,24 @@ Inductive expr :=
   | Lam2 (t : var) (e : expr)
   | App2 (e : expr) (tau : type)
   .
+
+Global Instance type_dec : EqDecision type.
+Proof. solve_decision. Qed.
+
+Instance type_countable : Countable type.
+Proof.
+ set (enc := fix go e :=
+  match e with
+  | Typ t => GenLeaf t
+  | Arr tau1 tau2 => GenNode 0 [go tau1; go tau2]
+  | All t tau => GenNode 1 [GenLeaf t; go tau]
+  end).
+ set (dec := fix go e :=
+  match e with
+  | GenLeaf t => Typ t
+  | GenNode 0 [tau1; tau2] => Arr (go tau1) (go tau2)
+  | GenNode 1 [GenLeaf t; tau] => All t (go tau)
+  | _ => Typ (xH)                  (* Dummy  *)
+  end).
+ refine (inj_countable' enc dec _). intros e. induction e; f_equal/=; auto.
+Qed.
